ROOT
@@ -1,4 +1,4 @@
-session LValues = "Lots-Of-Stuff" +
+session LValues = Bounded_Operators +
   options [quick_and_dirty = true]
   theories Laws
   document_files
